git-svn-id: https://projects.brucker.ch/hol-testgen/svn/HOL-TestGen/trunk/hol-testgen@10452 3260e6d1-4efc-4170-b0a7-36055960796d

src/OCL_tools.thy
@@ -44,4 +44,65 @@ theory OCL_tools
 imports OCL_core
 begin
 
+
+lemmas substs = OCL_core.foundation13[THEN iffD2, THEN OCL_core.StrongEq_L_subst2_rev]
+                OCL_core.foundation14[THEN iffD2, THEN OCL_core.StrongEq_L_subst2_rev]
+                OCL_core.foundation15[THEN iffD2, THEN OCL_core.StrongEq_L_subst2_rev]
+                OCL_core.foundation7'[THEN iffD2, THEN OCL_core.foundation15[THEN iffD2, 
+                                      THEN OCL_core.StrongEq_L_subst2_rev]]
+                OCL_core.StrongEq_L_subst2_rev
+
+                
+ML{*
+local val [c1,c2,c3,c4,c5] = @{thms "substs"}
+in
+
+fun ocl_subst_asm_tac ctxt x = FIRST[(etac c5 x) THEN (simp_tac ctxt x), 
+                                     (etac c4 x) THEN (simp_tac ctxt x), 
+                                     (etac c3 x) THEN (simp_tac ctxt x), 
+                                     (etac c2 x) THEN (simp_tac ctxt x),
+                                     (etac c1 x) THEN (simp_tac ctxt x)]
+end;
+
+val ocl_subst_asm = fn ctxt => SIMPLE_METHOD (ocl_subst_asm_tac ctxt 1); 
+
+val _ = Theory.setup 
+             (Method.setup (Binding.name "ocl_subst_asm") 
+             (Scan.succeed (ocl_subst_asm)) 
+             "ocl substition step") 
+ 
+*}
+
+lemma test1' : "\<tau> \<Turnstile> A \<Longrightarrow> \<tau> \<Turnstile> (A and B \<triangleq> B)"
+apply(tactic "ocl_subst_asm_tac @{context} 1")
+apply(simp)
+done
+
+lemma test1 : "\<tau> \<Turnstile> A \<Longrightarrow> \<tau> \<Turnstile> (A and B \<triangleq> B)"
+by(ocl_subst_asm, simp)
+
+lemma test2 : "\<tau> \<Turnstile> not A \<Longrightarrow> \<tau> \<Turnstile> (A and B \<triangleq> false)"
+by(ocl_subst_asm, simp)
+
+lemma test3 : "\<tau> \<Turnstile> (A \<triangleq> null) \<Longrightarrow> \<tau> \<Turnstile> (B \<triangleq> null) \<Longrightarrow> \<tau> \<Turnstile> not(A and B)"
+apply(ocl_subst_asm,ocl_subst_asm,simp)
+oops
+
+ (* TODO : establish support for goals of the form 
+   -  \<not> \<tau> \<Turnstile> A  
+   -  (\<tau> \<Turnstile> A)  = (\<tau> \<Turnstile> A')  
+   -  \<not>(\<tau> \<Turnstile> A)  = \<not>(\<tau> \<Turnstile> A')  
+   
+   Use :  OCL_core.StrongEq_L_subst3 etc...
+ *)
+
+ (* TODO : establish tactic support for ocl_subst thm1 ... thmn
+    (argument line version)
+ *)
+ 
+ (* TODO : Implement delta-closure procedure *)
+ 
+ (* TODO : Implement ocl_smt *)
+
+ 
 end
